Less memory allocation for MM

code/ecdsap256/Hacl.Impl.P256.MontgomeryMultiplication.fst
@@ -34,7 +34,7 @@ let add8_without_carry1 t t1 result  =
   let _  = add8 t t1 result in 
     assert_norm (pow2 320 + prime256 * prime256 < pow2 512)
 
-inline_for_extraction
+(* inline_for_extraction
 val montgomery_multiplication_round: t: widefelem -> round: widefelem -> Stack unit 
   (requires fun h -> live h t /\ live h round /\ wide_as_nat h t < prime256 * prime256)
   (ensures fun h0 _ h1 -> modifies (loc round)  h0 h1 /\
@@ -51,7 +51,38 @@ let montgomery_multiplication_round t round =
     shortened_mul prime256_buffer t1 t2;
     add8_without_carry1 t t2 t3;
     shift8 t3 round;
+  pop_frame()   *)
+
+inline_for_extraction
+val montgomery_multiplication_round: t: widefelem -> round: widefelem 
+  -> t2: lbuffer uint64 (size 8) 
+  -> t3: lbuffer uint64 (size 8) ->
+
+
+  Stack unit 
+  
+
+  (requires fun h -> live h t /\ live h round /\ wide_as_nat h t < prime256 * prime256)
+  (ensures fun h0 _ h1 -> modifies (loc round)  h0 h1 /\
+    wide_as_nat h1 round = (wide_as_nat h0 t + prime256 * (wide_as_nat h0 t % pow2 64)) / pow2 64
+  )
+
+let montgomery_multiplication_round t round t2 t3 =
+  push_frame(); 
+    let h0 = ST.get() in 
+(*     let t2 = create (size 8) (u64 0) in 
+    let t3 = create (size 8) (u64 0) in  *)
+    let t1 = mod64 t in 
+      recall_contents prime256_buffer (Lib.Sequence.of_list p256_prime_list); 
+    shortened_mul prime256_buffer t1 t2;
+    add8_without_carry1 t t2 t3;
+    shift8 t3 round;
   pop_frame()  
+
+
+
+
+
 
 
 val montgomery_multiplication_one_round_proof: 
@@ -69,7 +100,7 @@ let montgomery_multiplication_one_round_proof t result co =
   assert_norm (prime256 * prime256 > pow2 (575 - 64))
 
 
-inline_for_extraction noextract
+(* inline_for_extraction noextract
 val montgomery_multiplication_round_twice: t: widefelem -> result: widefelem -> Stack unit 
   (requires fun h -> live h t /\ live h result  /\ wide_as_nat h t < prime256 * prime256)
   (ensures fun h0 _ h1 -> 
@@ -82,7 +113,7 @@ val montgomery_multiplication_round_twice: t: widefelem -> result: widefelem -> 
     )
  )
 
-let montgomery_multiplication_round_twice t result = 
+let montgomery_multiplication_round_twice t result tempRound  = 
   assert_norm(prime256 > 3);
   push_frame();
     let tempRound = create (size 8) (u64 0) in 
@@ -94,7 +125,44 @@ let montgomery_multiplication_round_twice t result =
       let h2 = ST.get() in 
       montgomery_multiplication_one_round_proof (wide_as_nat h1 tempRound) (wide_as_nat h2 result) (wide_as_nat h0 t * modp_inv2_prime (pow2 64) prime256);
       lemma_montgomery_mod_inverse_addition (wide_as_nat h0 t);
+  pop_frame() *)
+
+
+
+inline_for_extraction noextract
+val montgomery_multiplication_round_twice: t: widefelem -> result: widefelem ->
+  tempRound: widefelem -> t2: widefelem -> t3: widefelem 
+
+
+-> Stack unit 
+  (requires fun h -> live h t /\ live h result  /\ wide_as_nat h t < prime256 * prime256)
+  (ensures fun h0 _ h1 -> 
+    modifies (loc result) h0 h1 /\
+    (
+      let round = (wide_as_nat h0 t + prime256 * (wide_as_nat h0 t % pow2 64)) / pow2 64 in 
+      wide_as_nat h1 result < prime256 * prime256 /\
+      wide_as_nat h1 result % prime256 == (wide_as_nat h0 t * modp_inv2_prime (pow2 128) prime256) % prime256 /\
+      wide_as_nat h1 result == (round + prime256 * (round % pow2 64)) / pow2 64
+    )
+ )
+
+let montgomery_multiplication_round_twice t result tempRound t2 t3  = 
+  assert_norm(prime256 > 3);
+  push_frame();
+    (* let tempRound = create (size 8) (u64 0) in  *)
+      let h0 = ST.get() in 
+    montgomery_multiplication_round t tempRound t2 t3; 
+      let h1 = ST.get() in 
+      montgomery_multiplication_one_round_proof (wide_as_nat h0 t)  (wide_as_nat h1 tempRound) (wide_as_nat h0 t);
+    montgomery_multiplication_round tempRound result t2 t3;
+      let h2 = ST.get() in 
+      montgomery_multiplication_one_round_proof (wide_as_nat h1 tempRound) (wide_as_nat h2 result) (wide_as_nat h0 t * modp_inv2_prime (pow2 64) prime256);
+      lemma_montgomery_mod_inverse_addition (wide_as_nat h0 t);
   pop_frame()
+
+
+
+
 
 inline_for_extraction noextract
 val montgomery_multiplication_buffer_by_one: a: felem -> result: felem ->  Stack unit
@@ -114,28 +182,33 @@ let montgomery_multiplication_buffer_by_one a result =
       let t_high = sub t (size 4) (size 4) in 
     let round2 = create (size 8) (u64 0) in 
     let round4 = create (size 8) (u64 0) in  
+
+    let t1 = create (size 8) (u64 0) in 
+    let t2 = create (size 8) (u64 0) in 
+    let t3 = create (size 8) (u64 0) in 
+
       let h0 = ST.get() in 
     copy t_low a; 
       let h1 = ST.get() in 
       assert(wide_as_nat h0 t = as_nat h0 t_low + as_nat h0 t_high * pow2 256);
       assert_norm (prime256 < prime256 * prime256);
-    montgomery_multiplication_round_twice t round2;
+    montgomery_multiplication_round_twice t round2 t1 t2 t3;
       let h2 = ST.get() in 
-    montgomery_multiplication_round_twice round2 round4; 
+    montgomery_multiplication_round_twice round2 round4 t1 t2 t3; 
       lemma_montgomery_mod_inverse_addition2 (wide_as_nat h1 t);
       lemma_mod_mul_distr_l (wide_as_nat h2 round2) (modp_inv2_prime (pow2 128) prime256) prime256;
       lemma_mod_mul_distr_l (wide_as_nat h1 t * modp_inv2_prime (pow2 128) prime256) (modp_inv2_prime (pow2 128) prime256) prime256;
-	mul_lemma_2 (wide_as_nat h1 t % pow2 64) (pow2 64 - 1) prime256;
-	mul_lemma_2 (let round = (wide_as_nat h1 t + prime256 * (wide_as_nat h1 t % pow2 64)) / pow2 64 in round % pow2 64) (pow2 64 - 1) prime256;
-	mul_lemma_2 (
-	  let round = (wide_as_nat h1 t + prime256 * (wide_as_nat h1 t % pow2 64)) / pow2 64 in  
-	  let round2 = (round + prime256 * (round % pow2 64)) / pow2 64 in 
-	  round2 % pow2 64) (pow2 64 - 1) prime256;
-	mul_lemma_2 (	
-	  let round = (wide_as_nat h1 t + prime256 * (wide_as_nat h1 t % pow2 64)) / pow2 64 in  
-	  let round2 = (round + prime256 * (round % pow2 64)) / pow2 64 in 
-	  let round3 = (round2 + prime256 * (round2 % pow2 64)) / pow2 64 in   
-	  round3 % pow2 64) (pow2 64 - 1) prime256;
+  mul_lemma_2 (wide_as_nat h1 t % pow2 64) (pow2 64 - 1) prime256;
+  mul_lemma_2 (let round = (wide_as_nat h1 t + prime256 * (wide_as_nat h1 t % pow2 64)) / pow2 64 in round % pow2 64) (pow2 64 - 1) prime256;
+  mul_lemma_2 (
+    let round = (wide_as_nat h1 t + prime256 * (wide_as_nat h1 t % pow2 64)) / pow2 64 in  
+    let round2 = (round + prime256 * (round % pow2 64)) / pow2 64 in 
+    round2 % pow2 64) (pow2 64 - 1) prime256;
+  mul_lemma_2 ( 
+    let round = (wide_as_nat h1 t + prime256 * (wide_as_nat h1 t % pow2 64)) / pow2 64 in  
+    let round2 = (round + prime256 * (round % pow2 64)) / pow2 64 in 
+    let round3 = (round2 + prime256 * (round2 % pow2 64)) / pow2 64 in   
+    round3 % pow2 64) (pow2 64 - 1) prime256;
     reduction_prime256_2prime256_8_with_carry_impl round4 result;
     lemmaFromDomain (as_nat h0 a);
   pop_frame()  
@@ -166,27 +239,36 @@ let montgomery_multiplication_buffer a b result =
     mul a b t;  
       let h1 = ST.get() in 
       mul_lemma_ (as_nat h0 a) (as_nat h0 b) prime256;
-  montgomery_multiplication_round_twice t round2;
+
+    let t1 = create (size 8) (u64 0) in 
+    let t2 = create (size 8) (u64 0) in 
+    let t3 = create (size 8) (u64 0) in 
+
+
+
+  montgomery_multiplication_round_twice t round2 t1 t2 t3;
       let h2 = ST.get() in 
-  montgomery_multiplication_round_twice round2 round4; 
+  montgomery_multiplication_round_twice round2 round4 t1 t2 t3; 
+
+
       let h3 = ST.get() in 
-	lemma_montgomery_mod_inverse_addition2 (wide_as_nat h1 t);
-	lemma_mod_mul_distr_l (wide_as_nat h2 round2) (modp_inv2_prime (pow2 128) prime256) prime256;
-	lemma_mod_mul_distr_l (wide_as_nat h1 t * modp_inv2_prime (pow2 128) prime256) (modp_inv2_prime (pow2 128) prime256) prime256;
+  lemma_montgomery_mod_inverse_addition2 (wide_as_nat h1 t);
+  lemma_mod_mul_distr_l (wide_as_nat h2 round2) (modp_inv2_prime (pow2 128) prime256) prime256;
+  lemma_mod_mul_distr_l (wide_as_nat h1 t * modp_inv2_prime (pow2 128) prime256) (modp_inv2_prime (pow2 128) prime256) prime256;
       mul_lemma_2 (wide_as_nat h1 t % pow2 64) (pow2 64 - 1) prime256;
       mul_lemma_ (as_nat h0 a) (as_nat h0 b) prime256;
       mul_lemma_1 ( 
          let round = (wide_as_nat h1 t + prime256 * (wide_as_nat h1 t % pow2 64)) / pow2 64 in  
-	 round % pow2 64) (pow2 64) prime256; 
+   round % pow2 64) (pow2 64) prime256; 
       mul_lemma_1 ( 
-	let round = (wide_as_nat h1 t + prime256 * (wide_as_nat h1 t % pow2 64)) / pow2 64 in 
-	let round2 = (round + prime256 * (round % pow2 64)) / pow2 64 in 
-	round2 % pow2 64) (pow2 64) prime256; 
+  let round = (wide_as_nat h1 t + prime256 * (wide_as_nat h1 t % pow2 64)) / pow2 64 in 
+  let round2 = (round + prime256 * (round % pow2 64)) / pow2 64 in 
+  round2 % pow2 64) (pow2 64) prime256; 
       mul_lemma_1 ( 
-	let round = (wide_as_nat h1 t + prime256 * (wide_as_nat h1 t % pow2 64)) / pow2 64 in 
-	let round2 = (round + prime256 * (round % pow2 64)) / pow2 64 in 
-	let round3 = (round2 + prime256 * (round2 % pow2 64)) / pow2 64 in 
-	round3 % pow2 64) (pow2 64) prime256;  
+  let round = (wide_as_nat h1 t + prime256 * (wide_as_nat h1 t % pow2 64)) / pow2 64 in 
+  let round2 = (round + prime256 * (round % pow2 64)) / pow2 64 in 
+  let round3 = (round2 + prime256 * (round2 % pow2 64)) / pow2 64 in 
+  round3 % pow2 64) (pow2 64) prime256;  
       assert_norm((prime256 * pow2 64 + (prime256 * pow2 64 + (prime256 * pow2 64 + ((pow2 64 - 1) * prime256 + prime256 * prime256) / pow2 64) / pow2 64)/ pow2 64) / pow2 64 < 2 * prime256);
   reduction_prime256_2prime256_8_with_carry_impl round4 result; 
   lemmaFromDomainToDomain (as_nat h0 a);
@@ -217,9 +299,16 @@ let montgomery_square_buffer a result =
     sq a t;  
       let h1 = ST.get() in 
       mul_lemma_ (as_nat h0 a) (as_nat h0 a) prime256;
-  montgomery_multiplication_round_twice t round2;
+
+    let t1 = create (size 8) (u64 0) in 
+    let t2 = create (size 8) (u64 0) in 
+    let t3 = create (size 8) (u64 0) in 
+
+
+
+  montgomery_multiplication_round_twice t round2 t1 t2 t3;
       let h2 = ST.get() in 
-  montgomery_multiplication_round_twice round2 round4; 
+  montgomery_multiplication_round_twice round2 round4 t1 t2 t3; 
       let h3 = ST.get() in 
   lemma_montgomery_mod_inverse_addition2 (wide_as_nat h1 t);
   lemma_mod_mul_distr_l (wide_as_nat h2 round2) (modp_inv2_prime (pow2 128) prime256) prime256;
